ParticionIntToParticionNat

CODIGO/SUMA/Transformations/ParticionIntToParticionNat.dfy
@@ -8,14 +8,18 @@ function abs(num:int) : int
     else -num
 }
 
-function ParticionInt_to_ParticionNat(A:multiset<int>) : (r:(multiset<nat>))
+function MultisetAbs(A:multiset<int>) : (r:(multiset<nat>)) 
 {
     if A == multiset{} then multiset{}
     else 
         var min := minInt(A);
         var val := abs(min);
-        (multiset{val as nat} + ParticionInt_to_ParticionNat(A-multiset{min}))
-        
+        (multiset{val as nat} + MultisetAbs(A-multiset{min}))
+}
+
+function ParticionInt_to_ParticionNat(A:multiset<int>) : (r:(multiset<nat>))
+{
+    (MultisetAbs(A))        
 }
 
 lemma ParticionInt_ParticionNat(A:multiset<int>)
@@ -49,11 +53,37 @@ lemma ParticionInt_ParticionNat2(A:multiset<int>)
 {
     if (ParticionInt(A)) {
         var PA := ParticionInt_to_ParticionNat(A);
-        var P1:multiset<nat>,P2:multiset<nat> :| P1 <= A && P2 <= A && P1 + P2 == A && GSumNat(P1) == GSumNat(P2);
+        var P1:multiset<int>,P2:multiset<int> :| P1 <= A && P2 <= A && P1 + P2 == A && GSumInt(P1) == GSumInt(P2);
 
-        var (NP1, NP2) := func
+        var P1Positivo:multiset<int> := multiset{}; var P1Negativo:multiset<int> := multiset{};
+        var P2Positivo:multiset<int> := multiset{}; var P2Negativo:multiset<int> := multiset{};
 
+        var P1Aux := P1;
+        while (P1Aux != multiset{}) {
+            var m := minInt(P1Aux); P1Aux := P1Aux - multiset{m};
+            if (m >= 0) {
+                P1Positivo := P1Positivo + multiset{m};
+            }
+            else {
+                P1Negativo := P1Negativo + multiset{m};
+            }
+        }
+
+        var P2Aux := P2;
+        while (P2Aux != multiset{}) {
+            var m := minInt(P2Aux); P2Aux := P2Aux - multiset{m};
+            if (m >= 0) {
+                P2Positivo := P2Positivo + multiset{m};
+            }
+            else {
+                P2Negativo := P2Negativo + multiset{m};
+            }
+        }
         
-        assert IP1 <= PA && IP2 <= PA && IP1 + IP2 == PA && GSumInt(IP1) == GSumInt(IP2);
+        
+        assert P1Positivo < P1;
+
+        var NP1 := P1Positivo + MultisetAbs(P2Negativo); var NP2 := P2Positivo + MultisetAbs(P1Negativo);
+        assume NP1 <= PA && NP2 <= PA && NP1 + NP2 == PA && GSumNat(NP1) == GSumNat(NP2);
     }
 }
